Fix lemmas of Unusedglob

backend/Unusedglob.v
@@ -122,6 +122,7 @@ Definition remove_gfun (gd : globdef fundef unit) :=
   |Gfun f => Gfun (Internal empty_function)
   end.
 
+(*
 Fixpoint filter_globdefs (used: IS.t) (accu defs: list (ident * globdef fundef unit)) :=
   match defs with
   | nil => accu
@@ -130,6 +131,16 @@ Fixpoint filter_globdefs (used: IS.t) (accu defs: list (ident * globdef fundef u
       then filter_globdefs (IS.remove id used) ((id, gd) :: accu) defs'
       else filter_globdefs used ((id, remove_gfun gd) :: accu) defs'
   end.
+ *)
+
+
+Definition filter_globdef (used: IS.t) (def: ident * globdef fundef unit) :=
+  match def with (id,gd) =>
+                   if IS.mem id used then (id,gd) else (id, remove_gfun gd)
+  end.
+
+Definition filter_globdefs (used: IS.t) (defs : list (ident * globdef fundef unit)) :=
+  map (filter_globdef used) defs.
 
 (** To ensure compatibility with linking, we must ensure that all the
   global names referenced are defined in the compilation unit, with
@@ -144,9 +155,27 @@ Definition transform_program (p: program) : res program :=
   | None => Error (msg "Unusedglob: analysis failed")
   | Some used =>
       if IS.for_all (global_defined p pm) used then
-        OK {| prog_defs := filter_globdefs used nil (List.rev p.(prog_defs));
+        OK {| prog_defs := filter_globdefs used p.(prog_defs);
               prog_public := p.(prog_public);
               prog_main := p.(prog_main) |}
       else
         Error (msg "Unusedglob: reference to undefined global")
   end.
+
+Lemma transform_skel : forall p tp, transform_program p = OK tp ->
+                     erase_program tp = erase_program p.
+Proof.
+  intros. unfold transform_program in H.
+  destruct used_globals; try discriminate.
+  destruct IS.for_all;try discriminate.
+  inv H.  unfold erase_program.
+  simpl. f_equal.
+  unfold filter_globdefs.
+  rewrite map_map.
+  eapply map_ext.
+  intros. destruct a. simpl.
+  destruct IS.mem.
+  - eauto.
+  - destruct g; simpl; reflexivity.
+Qed.
+        
